proof TT_EqDom_new done

theories/Environment/Stock.v
@@ -1,1114 +1,380 @@
-From Coq Require Import Lia.
-From Mecha Require Import Resource Resources Term Typ REnvironment 
-                          ResourcesMap Cell SREnvironment RContext.
-From DeBrLevel Require Import LevelInterface PairLevel.
+From Coq Require Import Lia List Arith.
+From Mecha Require Import Resource Term Triplet Evaluation_Transition REnvironment
+                          Cell.
+From DeBrLevel Require Import LevelInterface ListLevel.
 From MMaps Require Import MMaps.
-Import ResourceNotations ResourcesMapNotations 
-       TermNotations CellNotations REnvironmentNotations TypNotations
-       SREnvironmentNotations ResourcesNotations SetNotations RContextNotations.
+Import ResourceNotations TermNotations ListNotations REnvironmentNotations
+       CellNotations.
 
-(** * Environment - Virtual Resource Environment
-*)
-
-(** ** Module - Virtual Resource Environment *)
 Module Stock <: IsLvlET.
 
-Include IsLvlPairET SREnvironment ResourcesMap.
+Include IsLvlListETWL Triplet.
 
-Module RE := REnvironment.
-Module RC := RContext.
-Module SRE := SREnvironment.
-Module RM := ResourcesMap.
+Definition halts (m : lvl) (st : t) :=
+ List.Forall (fun (tp: Triplet.t) =>  let (_,v) := tp 
+                                      in Evaluation_Transition.halts m v) st.
 
-Open Scope renvironment_scope.
+Definition keys (st : t) :=
+ fold_right (fun '((rg,rs),_) acc => rg :: rs :: acc) [] st.
 
-(** *** Definitions *)
+Definition max_key (st : t) :=
+  fold_right (fun '((rg,rs),_) acc => max (max rg rs) acc) 0 st.
 
-(** **** Projections *)
-Definition readers (W : t) : 𝐄 := fst W.
-Definition writers (W : t) : RM.t := snd W.
-
-(** **** Empty stock 
-
-  A stock is empty if and only if both components are empty.
-*)
-Definition empty : t := (∅%sr,∅%rm). 
-
-Definition Empty (t : t) : Prop := SRE.Empty (readers t) /\ RM.Empty (writers t).
-
-Definition is_empty (t : t) : bool := SRE.Raw.is_empty (readers t) && RM.Raw.is_empty (writers t).
-
-(** **** Initialize the resource environment *)
-Definition init_locals (W : t) (V : 𝐕) : 𝐕 :=
-  SRE.init_readers (readers W) (RM.init_writers (writers W)  V).
-
-(** **** Update the resource environment 
-
-  For each instant, the resource environment is updated at the end. Each local resources may have a new initial term for the next instant. We defined [update_locals] which takes a stock [W] and a resource environment [V] and produces a new stock.
-*)
-Definition update_func (wW: RM.t) (V : 𝐕) (r: resource) (v: Λ) :=
-  match RM.find_data wW r with
-    | None => v
-    | Some rw =>  match V⌊rw⌋ with
-                      Some (⩽ … v' ⩾) =>  v'
-                    | _ => v
-                  end
+Definition new_key (st : t) :=
+  match st with
+    | [] => 0
+    | _  => (max_key st) + 1
   end.
 
-Definition update_readers_func (wW: RM.t) (V : 𝐕) (r: resource) (v: Λ) (rW: 𝐄) :=
-  match RM.find_data wW r with
-    | None => (⌈r ⤆ v⌉ rW)%sr
-    | Some rw =>  match V⌊rw⌋ with
-                      Some (⩽ … v' ⩾) =>  (⌈r ⤆ v'⌉ rW)%sr
-                    | _ => (⌈r ⤆ v⌉ rW)%sr
-                  end
+Fixpoint init_locals (st : t) (V : 𝐕) : 𝐕 :=
+  match st with
+    | [] => V
+    | (r,r',v) :: st' => (⌈r ⤆ ⩽ v … ⩾⌉(⌈r' ⤆ ⩽ unit … ⩾⌉ (init_locals st' V)))%re
   end.
 
-Definition update_readers (W: t) (V: 𝐕) :=
-  SRE.Raw.fold (update_readers_func (writers W) V) (readers W) (∅%sr).
+Fixpoint update_locals (st : t) (V : 𝐕) : t :=
+  match st with
+    | [] => []
+    | (r,r',v) :: st' =>  match (V⌊r'⌋)%re with
+                            | Some (⩽ … v' ⩾) =>  (r,r',v') :: (update_locals st' V)
+                            | _ => (r,r',v) :: (update_locals st' V)
+                          end
+  end.
 
-Definition update_locals (W : t) (V : 𝐕) : t := (update_readers W V, writers W).
-
-(** **** Add *)
-Definition add (rr rw : resource) (v : Λ) (W : t) : t :=
-  (⌈ rr ⤆ v ⌉ (readers W),(⌈rw ⤆ rr⌉ (writers W))%rm)%sr.
-
-(** **** Union
-
-  The union between two stocks is the point-to-point union between each component.
-*)
-Definition union (W W' : t) := ((readers W ∪ readers W')%sr, (writers W ∪ writers W')%rm).
-
-(** **** In
-
-  A resource name is in the stock if it is, at least, in one member of the stock.
-*)
-Definition In (r : resource) (W : t) := (r ∈ readers W)%sr \/ (r ∈ writers W)%rm.
-
-(** **** Find *)
-Definition find (r : resource) (W : t) := (readers W) ⌊r⌋%sr.
-
-(** **** Halts
-
-  In the functional transition proofs, we assume that all elements in the input resource environment halts. The resource environment depends on the stock for its initialization in the temporal transition. Consequently, we also need to define the halts property on the stock.
-*)
-Definition halts (k : lvl) (W : t) := SRE.halts k (readers W).
-
-(** **** New key *)
-
-Definition new_key (W : t) := max ((readers W)⁺)%sr ((writers W)⁺)%rm.
-
-(** **** Domain equality with [RContext] *)
-
-Definition eqDom (Rc : ℜ) (W: t) := forall (r : resource), (r ∈ Rc)%rc <-> In r W.
-
-Definition eqDom' (V : 𝐕) (W: t) := forall (r : resource), (r ∈ V)%re <-> In r W.
-
-(** *** Properties *)
-
-(** **** [Empty] properties *)
-
-Lemma Empty_empty : Empty empty.
-Proof.
-  split; simpl.
-  - apply SRE.empty_1.
-  - now apply RM.empty_1.
+Lemma halts_nil (m : lvl) : halts m [].
+Proof. 
+  unfold halts.
+  constructor.
 Qed.
 
-Lemma Empty_is_empty (t : t) : Empty t <-> is_empty t = true.
+Lemma halts_app (m : lvl) (st st' : t) :
+  halts m (st ++ st') <-> halts m st /\ halts m st'.
 Proof.
-  destruct t; unfold Empty, is_empty; simpl; split.
-  - intros [HE HE'].
-    apply SRE.is_empty_1 in HE; rewrite HE.
-    now apply RM.is_empty_1 in HE'; rewrite HE'.
-  - rewrite andb_true_iff. 
-    intros [HE HE'].
-    apply SRE.is_empty_2 in HE.
-    apply RM.is_empty_2 in HE'.
-    now split.
-Qed. 
-
-Lemma not_Empty_is_empty (t : t) : ~ Empty t <-> is_empty t = false.
-Proof.
-  split.
-  - intro HE.
-    apply not_true_is_false; intro Hc.
-    apply HE.
-    now rewrite Empty_is_empty.
-  - intros HE Hc.
-    revert HE.
-    apply eq_true_false_abs. 
-    now rewrite <- Empty_is_empty.
-Qed. 
-
-Lemma Empty_notin (t : t) : (forall r, ~ In r t) -> Empty t.
-Proof.
-  intros HnIn.
-  destruct t as [rt wt]; unfold In, Empty in *; simpl in *.
-  split.
-  - intros k v HM.
-    apply (HnIn k); left.
-    now exists v.
-  - intros k v HM.
-    apply (HnIn k); right.
-    now exists v.
+  unfold halts.
+  apply Forall_app.
 Qed.
 
-Lemma Empty_notin_1 (r : resource) (t : t) : Empty t -> ~ In r t.
+Lemma halts_weakening (m n : lvl) (st : t) : 
+  m <= n -> halts m st -> halts n (shift m (n - m) st).
 Proof.
-  unfold Empty, In; destruct t as [rt wt]; simpl.
-  intros [HEmp HEmp'] [[v HM] | [v HM]].
-  - apply (HEmp r v HM). 
-  - apply (HEmp' r v HM).
-Qed.
-
-Lemma Empty_unfold (t: t) : Empty t -> ~(exists r, In r t).
-Proof.
-  intros HEmp [].
-  revert H.
-  now apply Empty_notin_1.
-Qed.
-
-(** **** [init_locals] properties *)
-
-Lemma init_locals_in_iff (r : resource) (W : t) (V : 𝐕) :
-  (r ∈ (init_locals W V))%re <-> In r W \/ (r ∈ V)%re.
-Proof.
-  split; unfold init_locals, In; destruct W as [rW wW]; simpl.
-  - intro HIn. 
-    apply SRE.init_readers_in_iff in HIn as [| HIn]; auto.
-    apply RM.init_writers_in_iff in HIn as [|]; auto.
-  - intro HIns. 
-    apply SRE.init_readers_in_iff.
-    rewrite RM.init_writers_in_iff.
-    destruct HIns as [[HIn | HIn] | HIn]; auto.
-Qed.
-
-Lemma init_locals_find (r : resource) (v : 𝑣) (W : t) (V : 𝐕) :
- (init_locals W V)⌊r⌋%re = Some v -> In r W \/ V⌊r⌋%re = Some v.
-Proof.
-  unfold init_locals, In; destruct W as [rW wW]; simpl; intro Hfi. 
-  apply SRE.init_readers_find in Hfi as [| Hfi]; auto.
-  apply RM.init_writers_find in Hfi as [|]; auto.
-Qed.
-
-Lemma init_locals_find_1 (r : resource) (v : 𝑣) (W : t) (V : 𝐕) :
- (init_locals W V)⌊r⌋%re = Some v -> 
- (readers W)⌊r⌋%sr = Some (Cell.extract v) \/ 
- (RM.init_writers (writers W) V)⌊r⌋%re = Some v.
-Proof.
-  unfold init_locals, In; destruct W as [rW wW]; simpl; intro Hfi. 
-  apply SRE.init_readers_find_1 in Hfi as [| Hfi]; auto; right.
-Qed.
-
-Lemma init_locals_find_inp (rs : t) (V : 𝐕) (r : resource) (v : 𝑣) :
-  (forall r, V⌊r⌋%re = Some v -> exists v', Logic.eq v (Cell.inp v')) ->
-  ((init_locals rs V)⌊r⌋)%re = Some v -> exists v', Logic.eq v (Cell.inp v'). 
-Proof.
-  unfold init_locals; intros Ht Hfi.
-  apply SRE.init_readers_find_inp in Hfi; auto.
-  intros r' HfV.
-  apply RM.init_writers_find_inp in HfV; auto.
-Qed.
-
-Lemma init_locals_in_unused (W : t) (V : 𝐕) (r : resource) :
-  In r W -> RE.unused r (init_locals W V).
-Proof.
-  intro HIn; unfold In, init_locals in *; destruct W as [Rw Ww].
-  destruct HIn as [HIn | HIn]; simpl in *.
-  - now apply SRE.init_readers_in_unused.
-  - apply SRE.init_readers_unused. 
-    now apply RM.init_writers_in_unused.
-Qed.
-
-Lemma init_locals_unused (r : resource) (W : t) (V : 𝐕) :
-  RE.unused r V -> RE.unused r (Stock.init_locals W V).
-Proof.
-  unfold Stock.init_locals; intro Hunsd.
-  apply SRE.init_readers_unused.
-  now apply RM.init_writers_unused.
-Qed.
-
-Lemma init_locals_new_key (V : 𝐕) (t : t) : ((init_locals t V)⁺)%re = max (new_key t) (V⁺)%re.
-Proof.
-  destruct t; unfold init_locals, new_key; simpl.
-  rewrite SRE.init_readers_new_key.
-  rewrite RM.init_writers_new_key.
-  lia.
-Qed.
-
-(** **** [update_locals_readers] properties *)
-
-#[export] Instance sre_eq_equiv : Equivalence SREnvironment.eq := _.
-
-#[export] Instance update_readers_func_eq (wW: RM.t) (V: 𝐕) :
-  Proper (Logic.eq ==> Logic.eq ==> SRE.eq ==> SRE.eq) (update_readers_func wW V).
-Proof.
-  intros k' k Heqk v' v Heqv rW rW' HeqrW; subst.
-  unfold update_readers_func.
-  destruct (RM.find_data wW k).
-  - destruct (V⌊r⌋)%re.
-    -- destruct r0; now rewrite HeqrW.
-    -- now rewrite HeqrW.
-  - now rewrite HeqrW.
-Qed.
-
-Lemma update_readers_func_diamond (wW: RM.t) (V: 𝐕) :
-  SRE.Diamond SRE.eq (update_readers_func wW V).
-Proof.
-  intros k k' v v' rW rW1 rW1' Hneq Heq Heq'.
-  rewrite <- Heq, <- Heq'.
-  unfold update_readers_func.
-  destruct (RM.find_data wW k) eqn:Hfd.
-  - destruct (RM.find_data wW k') eqn:Hfd'.
-    -- destruct (V ⌊r⌋)%re eqn:Hfi.
-       + destruct (V ⌊r0⌋)%re eqn:Hfi'.
-         ++ destruct r1,r2;
-            now rewrite SRE.add_add_2; auto.
-         ++ destruct r1;
-            now rewrite SRE.add_add_2; auto.
-       + destruct (V ⌊r0⌋)%re.
-         ++ destruct r1;
-            now rewrite SRE.add_add_2; auto.
-         ++ now rewrite SRE.add_add_2; auto.
-    -- destruct (V ⌊r⌋)%re eqn:Hfi.
-       + destruct r0; now rewrite SRE.add_add_2; auto.
-       + now rewrite SRE.add_add_2; auto.
-  - destruct (RM.find_data wW k') eqn:Hfd'.
-    -- destruct (V ⌊r⌋)%re eqn:Hfi.
-       + destruct r0;
-         now rewrite SRE.add_add_2; auto.
-       + now rewrite SRE.add_add_2; auto.
-    -- now rewrite SRE.add_add_2; auto.
-Qed.
-
-Hint Resolve sre_eq_equiv update_readers_func_eq update_readers_func_diamond : core.
-
-Lemma update_readers_Empty_eq (W: t) (V: 𝐕) :
-  SRE.Empty (readers W) -> (update_readers W V = ∅)%sr.
-Proof.
-  intro HEmp; unfold update_readers.
-  rewrite SRE.fold_Empty; auto; reflexivity.
-Qed.
-
-Lemma update_readers_Empty (W: t) (V: 𝐕) : SRE.Empty (readers W) -> SRE.Empty (update_readers W V).
-Proof.
-  intro Hemp; unfold update_readers.
-  rewrite SRE.fold_Empty; now auto.
-Qed.
-
-Lemma update_readers_add (r: resource) (v: Λ) (rW: 𝐄) (wW: RM.t) (V: 𝐕) :
-  (r ∉ rW)%sr -> 
-  (update_readers (⌈r ⤆ v⌉ rW,wW) V = update_readers_func wW V r v (update_readers (rW,wW) V))%sr.
-Proof.
-  unfold update_readers; simpl.
-  intro HIn.
-  rewrite SRE.fold_Add with (e := v); eauto.
-  - reflexivity.
-  - unfold SRE.Add; reflexivity.
-Qed.
-
-Lemma update_readers_Add (r: resource) (v: Λ) (rW rW': 𝐄) (wW: RM.t) (V: 𝐕) :
-  (r ∉ rW)%sr -> SRE.Add r v rW rW' ->
-  (update_readers (rW',wW) V = update_readers_func wW V r v (update_readers (rW,wW) V))%sr.
-Proof.
-  unfold update_readers; simpl.
-  intros HIn Hadd.
-  now rewrite SRE.fold_Add with (e := v); eauto.
-Qed.
-
-Lemma update_readers_in_iff (r: resource) (W: t) (V: 𝐕) :
-  (r ∈ (update_readers W V))%sr <-> (r ∈ (readers W))%sr.
-Proof.
-  destruct W as [rW wW]; split; simpl.
-  - revert r.
-    induction rW using SRE.map_induction; intros r HIn.
-    -- rewrite update_readers_Empty_eq in HIn; auto.
-       inversion HIn.
-       apply SRE.empty_mapsto_iff in H0; inversion H0.
-    -- rewrite update_readers_Add in HIn; eauto.
-       unfold SRE.Add in H0; rewrite H0; clear H0.
-       rewrite SRE.add_in_iff.
-       unfold update_readers_func in HIn.
-       unfold update_readers_func.
-       destruct (RM.find_data wW);
-       try (destruct (V ⌊ r0 ⌋)%re);
-       try (destruct r1);
-       try (apply SRE.add_in_iff in HIn as [|]; now auto).
-  - revert r.
-    induction rW using SRE.map_induction; intros r HIn.
-    -- exfalso; destruct HIn.
-       now apply (H r x).
-    -- rewrite update_readers_Add; eauto.
-       unfold SRE.Add in H0; rewrite H0 in *; clear H0.
-       apply SRE.add_in_iff in HIn as [| HIn]; subst.
-       + unfold update_readers_func.
-         destruct (RM.find_data wW);
-         try (destruct (V ⌊ r0 ⌋)%re);
-         try (destruct r1);
-         try (rewrite SRE.add_in_iff; now auto).
-       + unfold update_readers_func.
-         destruct (RM.find_data wW);
-         try (destruct (V ⌊ r0 ⌋)%re);
-         try (destruct r1);
-         try (rewrite SRE.add_in_iff; now auto).
-Qed.
-
-Lemma update_readers_Empty' (W: t) (V: 𝐕) :
-  SRE.Empty (readers W) <-> SRE.Empty (update_readers W V).
-Proof.
-  split; intro.
-  - now apply update_readers_Empty.
-  - revert V H; destruct W as [rW wW]; simpl.
-    induction rW using SRE.map_induction; intros V HEmp; auto.
-    exfalso.
-    rewrite update_readers_Add in HEmp; eauto.
-    unfold update_readers_func in *.
-    destruct (RM.find_data wW x).
-    -- destruct ((V⌊r⌋)%re) eqn:Hfi.
-       + destruct r0.
-         ++ apply (HEmp x e).
-            apply SRE.add_mapsto_iff; auto.
-         ++ apply (HEmp x λ).
-            apply SRE.add_mapsto_iff; auto.
-       + apply (HEmp x e).
-         apply SRE.add_mapsto_iff; auto.
-    -- apply (HEmp x e).
-       apply SRE.add_mapsto_iff; auto.
-Qed.
-
-Lemma update_readers_new_key (V : 𝐕) (W: t) :
-  (update_readers W V)⁺%sr = (readers W⁺)%sr.
-Proof.
-  destruct W as [rW wW]; simpl in *.
-  induction rW using SRE.map_induction.
-  - rewrite update_readers_Empty_eq; auto.
-    symmetry.
-    do 2 (rewrite SRE.Ext.new_key_Empty; auto).
+  intro Hle.
+  induction st; intro Hlt.
   - simpl.
-    rewrite (update_readers_Add x e rW1); auto.
-    unfold SRE.Add in *; rewrite H0 in *; clear H0.
-    rewrite SRE.Ext.new_key_add_max, <- IHrW1.
-    unfold update_readers_func.
-    destruct (RM.find_data wW x);
-    try (destruct (V⌊r⌋)%re eqn:Hfi);
-    try (destruct r0);
-    try (now rewrite SRE.Ext.new_key_add_max).
+    constructor.
+  - simpl in *.
+    inversion Hlt; subst.
+    destruct a as [[rg rs] v].
+    constructor; simpl.
+    -- now apply Evaluation_Transition.halts_weakening.
+    -- now apply IHst.
 Qed.
 
-Lemma update_readers_Wf (k: lvl) (V : 𝐕) (W: t) :
-  (k ⊩ (readers W))%sr /\ (k ⊩ V)%re -> (k ⊩ (update_readers W V))%sr.
+
+Lemma keys_in_app (r : resource) (st st' : t) :
+  In r (keys (st ++ st')) <-> In r (keys st) \/ In r (keys st').
 Proof.
-  destruct W as [rW wW]; simpl.
-  intros [Hwf HwfV]; revert Hwf.
-  induction rW using SRE.map_induction; intro Hwf.
-  - rewrite update_readers_Empty_eq; auto.
-    apply SRE.Wf_empty.
-  - rewrite (update_readers_Add x e rW1); auto. 
-    unfold SRE.Add in H0; rewrite H0 in *; clear H0.
-    apply SRE.Wf_add_notin in Hwf as [Hwfx [Hwfe Hwf]]; auto.
-    unfold update_readers_func.
-    destruct (RM.find_data wW x);
-    try (destruct (V⌊r⌋)%re eqn:Hfi);
-    try (destruct r0);
-    try (apply SRE.Wf_add; now auto).
-    apply SRE.Wf_add; repeat split; auto.
-    apply (RE.Wf_find k) in Hfi as []; auto.
+  revert r st'; induction st; intros r st'.
+  - simpl; split; auto.
+    intros [|]; auto.
+    inversion H.
+  - destruct a as [[rg rs] v]; simpl; split.
+    -- intros [|[|HIn]]; subst; auto.
+       apply IHst in HIn; destruct HIn; auto.
+    -- intros [[|[|]]|]; subst; auto.
+       + do 2 right.
+         apply IHst; auto.
+       + do 2 right.
+         apply IHst; auto.
 Qed.
 
-(*
-update_readers_func (wW: RM.t) (V : 𝐕) (r: resource) (v: Λ) (rW: 𝐄) 
-*)
-Lemma update_readers_find (r: resource) (v v': Λ) (V: 𝐕) (W: t) :
-  (readers W)⌊r⌋%sr = Some v ->
-  (update_readers W V)⌊r⌋%sr = Some v' ->
-
-  v' = update_func (writers W) V r v.
+(* Lemma shift_in (m n : lvl) (tp : Triplet.t) (st : t) :
+  In tp st <-> In (Triplet.shift m n tp) (shift m n st).
 Proof.
-  unfold update_func.
-  destruct W as [rW wW]; simpl.
-  revert r v v' wW.
-  induction rW using SRE.map_induction. 
-  - intros r v v' wW Hfi Hfi'.
-    exfalso.
-    apply (H r v).
-    now apply SRE.find_2.
-  - intros r v v' wW Hfi Hfi'.
-    rewrite (update_readers_Add x e rW1 rW2) in Hfi'; auto.
-    destruct (Resource.eq_dec x r) as [| Hneq]; subst.
-    -- unfold SRE.Add in H0; rewrite H0 in Hfi; clear H0.
-       rewrite SRE.add_eq_o in Hfi; auto; inversion Hfi; subst. 
-       unfold update_readers_func in Hfi'.
-       destruct (RM.find_data wW r).
-       + destruct (V⌊r0⌋).
-         ++ destruct r1.
-            * rewrite SRE.add_eq_o in Hfi'; auto. 
-              inversion Hfi'; auto.
-            * rewrite SRE.add_eq_o in Hfi'; auto.
-              inversion Hfi'; auto.
-         ++ rewrite SRE.add_eq_o in Hfi'; auto. 
-            inversion Hfi'; auto.
-       + rewrite SRE.add_eq_o in Hfi'; auto. 
-         inversion Hfi'; auto.
-    -- unfold SRE.Add in H0; rewrite H0 in Hfi; clear H0.
-       rewrite SRE.add_neq_o in Hfi; auto.
-       unfold update_readers_func in Hfi'.
-       destruct (RM.find_data wW x).
-       + destruct (V⌊r0⌋).
-         ++ destruct r1.
-            * rewrite SRE.add_neq_o in Hfi'; auto.
-            * rewrite SRE.add_neq_o in Hfi'; auto.
-         ++ rewrite SRE.add_neq_o in Hfi'; auto.
-       + rewrite SRE.add_neq_o in Hfi'; auto.
+  revert r; induction st; simpl; intro r.
+  - split; auto.
+  - destruct a as [[rg rs] v]; simpl; split.
+    -- intros [|[|HIn]]; subst; auto.
+       do 2 right.
+       now apply IHst.
+    -- intros [|[|HIn]].
+       + apply Resource.shift_eq_iff in H; subst; auto.
+       + apply Resource.shift_eq_iff in H; subst; auto.
+       + apply IHst in HIn; auto.
+Qed. *)
+
+
+(* Lemma shift_in_e (m n : lvl) (tp : Triplet.t) (st : t) :
+  In tp (shift m n st) -> exists tp', Logic.eq tp (Triplet.shift m n tp').
+Proof.
+  revert tp; induction st; simpl; intro tp.
+  - intro Hc; inversion Hc.
+  - destruct a as [[rg rs] v]; simpl. intros [| HIn]; subst.
+    -- now exists (rg,rs,v).
+    -- auto.
+Qed. *)
+
+Lemma keys_in_shift (m n : lvl) (r : resource) (st : t) :
+  In r (keys st) <-> In ([⧐m – n] r)%r (keys (shift m n st)).
+Proof.
+  revert r; induction st; simpl; intro r.
+  - split; auto.
+  - destruct a as [[rg rs] v]; simpl; split.
+    -- intros [|[|HIn]]; subst; auto.
+       do 2 right.
+       now apply IHst.
+    -- intros [|[|HIn]].
+       + apply Resource.shift_eq_iff in H; subst; auto.
+       + apply Resource.shift_eq_iff in H; subst; auto.
+       + apply IHst in HIn; auto.
+Qed.
+
+Lemma keys_in_shift_e (m n : lvl) (r : resource) (st : t) :
+  In r (keys (shift m n st)) -> exists r', Logic.eq r ([⧐m – n] r')%r.
+Proof.
+  revert r; induction st; simpl; intro r.
+  - intro Hc; inversion Hc.
+  - destruct a as [[rg rs] v]; simpl; intros [|[| HIn]]; subst.
+    -- now exists rg.
+    -- now exists rs.
+    -- auto.
+Qed.
+
+Lemma keys_in_new_key (r : resource) (st : t) :
+  In r (keys st) -> r < (new_key st).
+Proof.
+  revert r; induction st; intro r.
+  - simpl; lia.
+  - destruct a as [[rg rs] v]; simpl.
+    intros [|[|HIn]]; subst; try lia.
+    apply IHst in HIn.
+    destruct st.
+    simpl in *; try lia.
+    unfold new_key in HIn.
+    lia.
+Qed.
+
+Lemma max_key_app (st st' : t) :
+  max_key (st ++ st') = max (max_key st) (max_key st').
+Proof.
+  induction st.
+  - now simpl.
+  - destruct a as [[rg rs] v].
+    simpl.
+    rewrite IHst.
+    lia.
+Qed.
+
+Lemma new_key_app (st st' : t) :
+  new_key (st ++ st') = max (new_key st) (new_key st').
+Proof.
+  unfold new_key.
+  destruct st.
+  - now simpl.
+  - destruct p as [[rg rs] v].
+    simpl.
+    rewrite max_key_app.
+    destruct st'; simpl.
+    -- lia.
+    -- destruct p as [[rg' rs'] v'].
+       lia.
+Qed.
+
+Lemma new_key_cons (r r' : resource) (v : Λ) (st : t) :
+  new_key ((r,r',v) :: st) = max (r + 1) (max (r' + 1) (new_key st)).
+Proof.
+  destruct st.
+  - simpl; lia.
+  - destruct p as [[rg rs] v']; simpl; lia.
 Qed. 
 
-(** **** [update_locals] properties *)
-
-Lemma update_locals_in_iff (r : resource) (W : t) (V : 𝐕) :
-  In r (update_locals W V) <-> In r W.
+Lemma max_key_shift_refl (m n : lvl) (st : t) :
+  m >= (new_key st) -> max_key (shift m n st) = max_key st.
 Proof.
-  split; unfold init_locals, In; destruct W as [rW wW]; simpl.
-  - intros [HIn |]; auto. 
-    apply update_readers_in_iff in HIn; auto.
-  - intros [HIn |]; auto; left. 
-    now apply update_readers_in_iff.
+  induction st.
+  - simpl; auto.
+  - destruct a as [[rg rs] v]; simpl; intros.
+    rewrite <- IHst.
+    -- f_equal.
+       rewrite Resource.shift_wf_refl.
+       + rewrite Resource.shift_wf_refl; auto.
+         unfold Resource.Wf; lia.
+       + unfold Resource.Wf; lia.
+    -- destruct st.
+       + simpl; lia.
+       + destruct p as [[rg' rs'] v']. simpl in *; lia.
 Qed.
 
-Lemma update_locals_Empty (t: t) (V: 𝐕) :
-  Empty (update_locals t V) <-> Empty t.
+Lemma new_key_shift_refl (m n : lvl) (st : t) :
+  m >= (new_key st) -> new_key (shift m n st) = new_key st.
 Proof.
-  unfold update_locals, Empty.
-  destruct t as [rt wt]; simpl; split.
-  - intros [HEmp ]; split; auto.
-    rewrite <- (update_readers_Empty' _ V) in HEmp; auto.
-  - intros [HEmp ]; split; auto.
-    now apply update_readers_Empty.
+  destruct st.
+  - now simpl.
+  - destruct p as [[rg rs] v].
+    simpl.
+    intros.
+    rewrite max_key_shift_refl; try lia.
+    -- f_equal. f_equal.
+       rewrite Resource.shift_wf_refl.
+       + rewrite Resource.shift_wf_refl; auto.
+         unfold Resource.Wf; lia.
+       + unfold Resource.Wf; lia.
+    -- destruct st; simpl; try lia.
+       destruct p as [[rg' rs'] v'].
+       simpl in *; lia.
+Qed.
+
+Lemma keys_in_shift_new_key (n : lvl) (r : resource) (st : t) :
+  In r (keys (shift (new_key st) n st)) <-> In r (keys st).
+Proof.
+  split; intro HIn.
+  - apply keys_in_shift_e in HIn as Heq.
+    destruct Heq as [r' ]; subst.
+    apply keys_in_shift in HIn.
+    apply keys_in_new_key in HIn as Hlt.
+    rewrite Resource.shift_wf_refl; auto.
+  - apply keys_in_new_key in HIn as Hlt.
+    rewrite <- (Resource.shift_wf_refl (new_key st) n r); auto.
+    now rewrite <- keys_in_shift.
+Qed.
+
+Lemma NoDup_keys_app (st st' : t) :
+  NoDup (keys st) -> NoDup (keys st') ->
+  (forall r, In r (keys st') -> ~ In r (keys st)) ->
+  NoDup (keys (st ++ st')).
+Proof.
+ revert st'; induction st; intros st' HNoD1 HNoD2 Hdisj.
+ - now simpl.
+ - destruct a as [[rg rs] v]; simpl in *.
+   inversion HNoD1; subst. 
+   simpl in *.
+   inversion H2; subst.
+   constructor.
+   -- simpl; intros [| HIn]; subst.
+      + apply H1; now left.
+      + apply keys_in_app in HIn; destruct HIn as [HIn|HIn].
+        ++ apply H1; auto.
+        ++ apply Hdisj in HIn.
+           apply HIn; auto.
+   -- constructor.
+      + intro HIn.
+        apply keys_in_app in HIn; destruct HIn as [HIn|HIn].
+        ++ auto.
+        ++ apply Hdisj in HIn.
+           apply HIn; auto.
+      + apply IHst; auto.
+        intros r HIn.
+        apply Hdisj in HIn; auto.
+Qed.
+
+Lemma NoDup_keys_shift (m n : lvl) (st : t) :
+  NoDup (keys st) -> NoDup (keys (shift m n st)).
+Proof.
+  induction st.
+  - simpl; auto.
+  - destruct a as [[rg rs] v]; simpl.
+    intro HNoD.
+    inversion HNoD; subst.
+    inversion H2; subst.
+    constructor.
+    -- simpl; intros [|HIn].
+       + apply Resource.shift_eq_iff in H; subst.
+         apply H1.
+         simpl; auto.
+       + apply keys_in_shift in HIn.
+         apply H1; simpl; auto.
+    -- constructor; auto.
+       simpl in *.
+       now rewrite <- keys_in_shift.
+Qed.
+
+Lemma update_locals_max_key (V : 𝐕) (t : t) :
+  max_key (update_locals t V) = max_key t.
+Proof.
+  induction t; simpl; auto.
+  destruct a as [[rg rs] v]; subst.
+  destruct (V⌊rs⌋)%re as [ov|]; try (destruct ov); 
+  simpl; now rewrite IHt.
 Qed.
 
 Lemma update_locals_new_key (V : 𝐕) (t : t) :
   new_key (update_locals t V) = new_key t.
 Proof.
-  destruct t; unfold update_locals, new_key; simpl.
-  rewrite update_readers_new_key; simpl; lia.
+  unfold new_key.
+  destruct t; simpl; auto.
+  destruct p as [[rg rs] v].
+  destruct (V⌊rs⌋)%re as [ov|]; try (destruct ov); 
+  simpl; now rewrite update_locals_max_key.
+Qed.
+
+Lemma Wf_cons_1 (k : lvl) p (t : t) :
+  Wf k (p :: t) -> Wf k t.
+Proof.
+  intros Hwf r HIn; apply Hwf; simpl; auto.
 Qed.
 
 Lemma update_locals_Wf (k: lvl) (V : 𝐕) (W: t) :
   Wf k W /\ (k ⊩ V)%re -> Wf k (update_locals W V).
 Proof.
-  destruct W as [rW wW].
-  unfold Wf, update_locals; simpl.
-  intros [[Hwfr Hwfw] HwfV].
-  split; auto.
-  apply update_readers_Wf; auto.
+  induction W; simpl; intros [Hwf Hwf']; auto.
+  destruct a as [[rg rs] v].
+  apply Wf_cons in Hwf as [Hwf Hwf''].
+  destruct (V⌊rs⌋)%re eqn:Hfi; try (destruct r); 
+  intro r; simpl; intros [|HIn]; subst;
+  try (apply IHW; auto; split; now auto);
+  try (apply Hwf; simpl; now auto).
+  destruct Hwf.
+  eapply REnvironment.Wf_find in Hfi; eauto.
+  simpl in *; destruct Hfi.
+  unfold Cell.Wf in *; simpl in *.
+  repeat split; auto.
 Qed.
 
-Lemma update_locals_find (r: resource) (v: Λ) (V: 𝐕) (W: t) :
-  find r (update_locals W V) = Some v ->
-  exists v',
-    (readers W)⌊r⌋%sr = Some v' /\
-    v = update_func (writers W) V r v'.
+Lemma halts_init_locals (m : lvl) (st : t) (V : 𝐕) :
+  halts m st -> REnvironment.halts m V -> 
+  REnvironment.halts m (init_locals st V).
 Proof.
-  unfold find, update_locals.
-  destruct W as [rW wW]; simpl.
-  intro Hfi.
-  assert (HIn: (r ∈ readers (rW,wW))%sr).
-  { 
-    rewrite <- (update_readers_in_iff _ _ V). 
-    exists v; now apply SRE.find_2. 
-  }
-  destruct HIn as [v' Hfi'].
-  apply SRE.find_1 in Hfi'.
-  exists v'; split; auto.
-  apply (update_readers_find _ v') in Hfi; auto.
-Qed.
-
-(* Lemma update_locals_union (r: resource) (v: Λ) (V: 𝐕) (W W': t) :
-  find r (update_locals (union W W') V) = Some v <->
-  find r (union (update_locals W V) (update_locals W' V)) = Some v.
-Proof.
-  unfold find, update_locals; simpl.
-  destruct W,W'; simpl.
-  revert r v V W'.
-*)
-
-(** **** [In] properties  *)
-
-Lemma empty_in (r : resource) : ~ In r empty.
-Proof.
-  unfold In, empty; simpl; intros [HIn | HIn].
-  - revert HIn; apply SRE.not_in_empty.
-  - revert HIn; apply RM.not_in_empty.
-Qed.
-
-Lemma add_in_iff (r r' k : resource) (v : Λ) (W : t) :
-  In k (add r r' v W) <-> k = r \/ k = r' \/ In k W.
-Proof.
-  unfold add, In; destruct W as [rw wW]; simpl; split.
-  - intros [HIn | HIn].
-    -- destruct (Resource.eq_dec k r) as [| Hneq]; subst; auto. 
-       rewrite SRE.add_neq_in_iff in HIn; auto.
-    -- destruct (Resource.eq_dec k r') as [| Hneq]; subst; auto. 
-       rewrite RM.add_neq_in_iff in HIn; auto.
-  - rewrite SRE.add_in_iff; rewrite RM.add_in_iff.
-    intros [Heq | [Heq | [HIn | HIn]]]; subst; auto.
-Qed.
-
-Lemma union_in_iff (r : resource) (W W' : t) : 
-  In r (union W W') <-> In r W \/ In r W'.
-Proof.
-  unfold In,union; destruct W,W'; simpl.
-  rewrite SRE.extend_in_iff; rewrite RM.extend_in_iff.
-  split; intros [[|] | [|]]; auto.
-Qed.
-
-Lemma In_dec (r: resource) (W: t) : {In r W} + {~ In r W}.
-Proof.
-  destruct W as [rW wW]; unfold In; simpl.
-  destruct (SRE.In_dec rW r) as [HInrW | HnInrW];
-  destruct (RM.In_dec wW r) as [HInwW | HnInwW]; auto.
-  right; intros [|]; auto.
-Qed.
-
-Lemma Empty_union (t1 t2: t) : Empty (union t1 t2) <-> (Empty t1) /\ (Empty t2).
-Proof.
-  split.
-  - intros HEmp.
-    apply Empty_unfold in HEmp; split.
-    -- apply Empty_notin; intros r HIn.
-       apply HEmp.
-       exists r.
-       rewrite union_in_iff; auto.
-    -- apply Empty_notin; intros r HIn.
-       apply HEmp.
-       exists r.
-       rewrite union_in_iff; auto.
-  - intros [HEmp1 HEmp2].
-    apply Empty_unfold in HEmp1,HEmp2.
-    apply Empty_notin.
-    intros r HIn.
-    apply union_in_iff in HIn as [|].
-    -- apply HEmp1.
-       now exists r.
-    -- apply HEmp2.
-       now exists r.
-Qed.
-
-(** **** [find] properties *)
-
-Lemma find_union (r : resource) (v : Λ) (W W' : t) :
-  find r (union W W') = Some v -> find r W = Some v \/ find r W' = Some v.
-Proof.
-  unfold find, union; destruct W,W'; simpl; intro HM.
-  apply SRE.find_2 in HM. 
-  apply SRE.extend_mapsto_iff in HM as [HM | [HM _]];
-  apply SRE.find_1 in HM; auto.
-Qed.
-
-Lemma find_add_eq (r r': resource) (v: Λ) (W: t) :
-  find r (add r r' v W) = Some v.
-Proof.
-  unfold find, add; destruct W; simpl.
-  now apply SRE.add_eq_o.
-Qed. 
-
-Lemma find_add_neq (r r' r'': resource) (v: Λ) (W: t) :
-  r <> r'' -> find r'' (add r r' v W) = find r'' W.
-Proof.
-  unfold find, add; destruct W; simpl; intro.
-  now apply SRE.add_neq_o.
-Qed. 
-
-
-(** **** [Wf] poperties *)
-
-Lemma Wf_empty (k : lvl) : Wf k empty.
-Proof.
-  unfold Wf, empty; simpl; split.
-  - apply SRE.Wf_empty.
-  - apply RM.Wf_empty.
-Qed.
-
-Lemma Wf_Empty (k : lvl) (t : t) : Empty t -> Wf k t.
-Proof.
-  unfold Wf, Empty; destruct t; simpl; split.
-  - destruct H.
-    now apply SRE.Wf_Empty.
-  - destruct H.
-    now apply RM.Wf_Empty.
-Qed.
-
-Lemma Wf_add (k : lvl) (r r' : resource) (v : Λ) (W : t) :
-  (k ⊩ r)%r -> (k ⊩ r')%r -> (k ⊩ v)%tm -> Wf k W -> Wf k (add r r' v W).
-Proof.
-  unfold Wf; destruct W as [rW wW]; simpl. 
-  intros Hvr Hvr' Hvv [HvrW HvwW]; split.
-  - apply SRE.Wf_add; auto.
-  - apply RM.Wf_add; auto.
-Qed.
-
-Lemma Wf_union (k : lvl) (W W' : t) :
-  Wf k W /\ Wf k W' -> Wf k (union W W').
-Proof.
-  unfold Wf; destruct W,W'; simpl. 
-  intros [[HvrW HvwW] [HvrW' HvwW']]; split.
-  - apply SRE.Wf_extend; auto.
-  - apply RM.Wf_extend; auto.
-Qed.
-
-Lemma Wf_in (k : lvl) (r : resource) (W : t) :
-  In r W -> Wf k W -> (k ⊩ r)%r.
-Proof.
-  unfold In, Wf; destruct W as [rW wW]; simpl.
-  intros [HIn | HIn] [HvrW HvwW].
-  - eapply SRE.Wf_in in HIn; eauto.
-  - eapply RM.Wf_in; eauto.
-Qed.
-
-Lemma Wf_in_iff (m n k : lvl) (W : t) :
-  Wf m W -> In k (shift m n W) <-> In k W.
-Proof.
-  unfold Wf, shift, In; destruct W as [rW wW]; simpl.
-  intros [Hvr Hvw]; split; intros [HIn | HIn].
-  - now left; rewrite SRE.Wf_in_iff in HIn.
-  - now right; rewrite RM.Wf_in_iff in HIn.
-  - now left; rewrite SRE.Wf_in_iff.
-  - now right; rewrite RM.Wf_in_iff.
-Qed.
-
-Lemma init_locals_Wf (k : lvl) (V : 𝐕) (t : t) :
-  Wf k t /\ (k ⊩ V)%re -> (k ⊩ init_locals t V)%re.
-Proof.
-  destruct t as [rW wW]. 
-  intros [[HvrW HvrwW] HvV].
-  simpl in *. unfold init_locals.
-  apply SRE.init_readers_Wf; simpl; split; auto.
-  apply RM.init_writers_Wf; simpl; split; auto.
-Qed.
-
-(** **** [new_key] properties *)
-
-Lemma new_key_empty : new_key empty = 0.
-Proof.
-  unfold new_key, empty.
-  simpl (readers (∅, ∅%rm) ⁺)%sr.
-  simpl (writers (∅%sr, ∅) ⁺)%rm.
-  rewrite SRE.Ext.new_key_empty. 
-  rewrite RM.Ext.new_key_empty.
-  now simpl. 
-Qed.
-
-Lemma new_key_Empty (t : t) : Empty t -> new_key t = 0.
-Proof.
-  destruct t; intros []; simpl in *.
-  unfold new_key; simpl.
-  rewrite SRE.Ext.new_key_Empty; auto.
-  rewrite RM.Ext.new_key_Empty; auto.
-Qed.
-
-Lemma new_key_in (r: lvl) (t : t) : 
-  In r t -> (r < new_key t)%nat.
-Proof.
-  destruct t as [rt wt].
-  unfold In, new_key; simpl.
-  intros [HIn | HIn].
-  - apply SRE.Ext.new_key_in in HIn; lia.
-  - apply RM.Ext.new_key_in in HIn; lia.
-Qed.
-
-Lemma new_key_union (t1 t2: t) :
-  new_key (union t1 t2) = max (new_key t1) (new_key t2).
-Proof.
-  unfold new_key, union; destruct t1, t2; simpl.
-  rewrite SRE.extend_new_key.
-  rewrite RM.extend_new_key.
-  lia.
-Qed.
-
-Lemma new_key_Wf (k: lvl) (t: t) : Wf k t -> new_key t <= k.
-Proof.
-  unfold Wf, new_key; destruct t; simpl.
-  intros [Hwf Hwf'].
-  apply SRE.new_key_Wf in Hwf.
-  apply RM.new_key_Wf in Hwf'.
-  lia.
-Qed. 
-
-Lemma new_key_add_max (m n: lvl) (v: Λ) (t: t) : 
-  new_key (add m n v t) = max (S m) (max (S n) (new_key t)).
-Proof.
-  destruct t; unfold new_key, add. 
-  simpl (readers (⌈ m ⤆ v ⌉ readers (t0, t1), (⌈n ⤆ m⌉  writers (t0, t1))%rm))%sr.
-  simpl (writers ((⌈ m ⤆ v ⌉ readers (t0, t1))%sr, (⌈n ⤆ m⌉  writers (t0, t1))%rm)).
-  simpl (readers (t0, t1)).
-  simpl (writers (t0, t1)).
-  rewrite SRE.Ext.new_key_add_max.
-  rewrite RM.Ext.new_key_add_max; lia.
-Qed.
-
-
-(** **** [shift] properties *)
-
-
-Lemma shift_new_refl (lb k : lvl) (t : t) :
-  lb >= (new_key t) -> new_key (shift lb k t) = new_key t.
-Proof.
-  unfold new_key, shift; destruct t; simpl.
-  intro Hgeq.
-  rewrite SRE.shift_new_refl; try lia.
-  rewrite RM.shift_new_refl; lia.
-Qed.
-
-Lemma shift_in_iff (m n : lvl) (r : resource) (W : t) :
-  In r W <-> In ([⧐ m – n] r)%r (shift m n W).
-Proof.
-  unfold In, shift; destruct W as [rW wW]; simpl; 
-  split; intros [HIn | HIn].
-  - left. now apply SRE.shift_in_iff.
-  - right; now apply RM.shift_in_iff.
-  - left. rewrite SRE.shift_in_iff; eauto.
-  - right; rewrite RM.shift_in_iff; eauto.
-Qed.
-
-Lemma shift_in_e (m n : lvl) (r : resource) (W : t) :
-  In r (shift m n W) -> exists r', (r =  ([⧐ m – n] r')%r)%type.
-Proof.
-  unfold In,shift; destruct W as [rW wW]; simpl; intros [HIn | HIn].
-  - apply SRE.shift_in_e in HIn; auto.
-  - apply RM.shift_in_e in HIn; auto.
-Qed.
-
-Lemma shift_Empty_iff (m n: lvl) (W: t) :
-  Empty W <-> Empty (shift m n W).
-Proof.
-  split; intro HEmp.
-  - apply Empty_unfold in HEmp.
-    apply Empty_notin; intros r HIn.
-    apply shift_in_e in HIn as HI.
-    destruct HI as [r']; subst.
-    rewrite <- shift_in_iff in HIn.
-    apply HEmp.
-    now exists r'.
-  - apply Empty_unfold in HEmp.
-    apply Empty_notin; intros r HIn.
-    rewrite (shift_in_iff m n) in HIn.
-    apply HEmp.
-    now exists ([⧐m – n] r)%r.
-Qed.
-
-Lemma shift_new_key_in_iff (n : lvl) (x : resource) (t : t) :
-  In x (shift (new_key t) n t) <-> In x t.
-Proof.
-  split; intro HIn.
-  - apply shift_in_e in HIn as H.
-    destruct H as [y Heq]; subst.
-    rewrite <- shift_in_iff in HIn.
-    apply new_key_in in HIn as Hlt.
-    rewrite Resource.shift_wf_refl; auto.
-  - apply new_key_in in HIn as Hlt.
-    rewrite <- (Resource.shift_wf_refl (new_key t) n x); auto.
-    now rewrite <- shift_in_iff.
-Qed.
-
-Lemma shift_find_iff (k n : lvl) (r: resource) v (t : t) :
-  find r t = Some v <-> find ([⧐ k – n] r)%r (shift k n t) = Some (<[[⧐ k – n] v]>)%tm.
-Proof.
-  unfold shift, find; destruct t; simpl.
-  apply SRE.shift_find_iff.
-Qed.
-
-Lemma shift_find_e_1 (k n : lvl) (r: resource) v (t : t) :
-  find r (shift k n t) = Some v -> (exists r', (r = ([⧐ k – n] r')%r)%type) /\
-                                   (exists v', (v = <[[⧐ k – n] v']>%tm)%type).
-Proof.
-  unfold find, shift; destruct t; simpl.
-  intros Hfi.
-  apply SRE.shift_find_e_1 in Hfi; auto.
-Qed.
-
-(** **** [halts] properties *)
-
-#[export] Instance halts_eq: Proper (Logic.eq ==> eq ==> iff) halts.
-Proof.
-  unfold halts; intros k' k Heqk W W' Heqst; subst.
-  destruct W,W'; repeat red in Heqst; unfold RelationPairs.RelCompFun in Heqst;
-  simpl in *; destruct Heqst as [HeqR _].
-  now rewrite HeqR.
-Qed.
-
-Lemma halts_init_locals (k : lvl) (W : t) (V : 𝐕) :
-  halts k W -> RE.halts k V -> RE.halts k (init_locals W V).
-Proof.
-  unfold halts, init_locals; destruct W as [rW wW]; simpl.
-  intros HvrW HvV.
-  apply SRE.halts_init_readers; auto.
-  now apply RM.halts_init_writers.
-Qed.
-
-Lemma halts_update_readers (k : lvl) (W: t) (V: 𝐕) :
-  SRE.halts k (readers W) -> RE.halts k V -> SRE.halts k (update_readers W V).
-Proof.
-  destruct W as [rW wW]; simpl.
-  induction rW using SRE.map_induction; intros Hltrs HltV.
-  - now rewrite update_readers_Empty_eq.
-  - rewrite (update_readers_Add x e rW1); auto. 
-    unfold SREnvironment.Add in H0; rewrite H0 in *; clear H0.
-    apply SRE.halts_add_iff in Hltrs as [Hlte Hltrw1]; auto.
-    specialize (IHrW1 Hltrw1 HltV).
-    unfold update_readers_func.
-    destruct (RM.find_data wW x);
-    try (destruct ((V⌊r⌋)%re) eqn:Hfi);
-    try (destruct r0);
-    try (rewrite SRE.halts_add_iff; try now split);
-    try (now rewrite update_readers_in_iff; simpl).
-    split; auto.
-    apply HltV in Hfi; now simpl.
+  induction st.
+  - simpl; intros.
+    intros k v Hfi.
+    now apply H0 in Hfi.
+  - intros Hlt HltV.
+    destruct a as [[rg rs] v'].
+    simpl.
+    inversion Hlt; subst.
+    apply IHst in H2; auto.
+    apply REnvironment.halts_add; split.
+    -- now simpl.
+    -- apply REnvironment.halts_add; split; auto.
+       simpl.
+       exists <[unit]>; split; auto.
+       reflexivity.
 Qed.
 
 Lemma halts_update_locals (k : lvl) (W : t) (V : 𝐕) :
-  RE.halts k V -> halts k W -> halts k (update_locals W V).
+  REnvironment.halts k V -> halts k W -> halts k (update_locals W V).
 Proof.
-  intros HltV HltW; unfold halts,update_locals.
-  destruct W as [Rw Ww]; simpl.
-  apply halts_update_readers; auto.
-Qed.
-
-
-Lemma halts_weakening (m n : lvl) (W : t) : 
-  m <= n -> halts m W -> halts n (shift m (n - m) W).
-Proof.
-  unfold halts, shift; destruct W as [rW wW]. 
-  simpl; intros Hle HvrW.
-  now apply SRE.halts_weakening.
-Qed.
-
-Lemma halts_union (k : lvl) (W W' : t) :
-  halts k W /\ halts k W' -> halts k (union W W').
-Proof.
-  unfold halts; destruct W,W'; simpl; intro Hlt. 
-  now apply SRE.halts_union.
-Qed.
-
-Lemma halts_add (k : lvl) (r r' : resource) (v : Λ) (W : t) :
-  (Evaluation_Transition.halts k v) /\ halts k W -> halts k (add r r' v W).
-Proof.
-  unfold halts, add; destruct W as [rW wW]; simpl; intro Hv.
-  now apply SRE.halts_add.
-Qed.
-
-Lemma halts_Empty (k: resource) (t: t) : Empty t -> halts k t.
-Proof.
-  destruct t as [rt wt]; unfold Empty, halts; simpl.
-  intros [HEmp _].
-  now apply SRE.halts_Empty.
-Qed.
-
-(** **** Morphisms *)
-
-
-#[export] Instance stock_in_iff : Proper (Logic.eq ==> eq ==> iff) In.
-Proof.
-  unfold eq, In; intros k' k Heqk W W' Heqst; subst.
-  destruct W,W'; repeat red in Heqst; unfold RelationPairs.RelCompFun in Heqst;
-  simpl in *; destruct Heqst as [HeqR HeqW].
-  now rewrite HeqR, HeqW.
-Qed.
-
-#[export] Instance stock_find_eq : Proper (Logic.eq ==> eq ==> Logic.eq) find.
-Proof.
-  unfold find, eq; intros k' k Heqk W W' Heqst; subst.
-  destruct W,W'; repeat red in Heqst; unfold RelationPairs.RelCompFun in Heqst;
-  simpl in *; destruct Heqst as [HeqR HeqW].
-  now rewrite HeqR.
-Qed.
-
-#[export] Instance stock_add_eq : Proper (Resource.eq ==> Resource.eq ==> Term.eq ==> eq ==> eq) add.
-Proof.
-  unfold eq, add.
-  intros r' r Heqr r1' r1 Heqr1 d d' Heqd W W' Heqst; destruct W,W'. 
-  repeat red in Heqst; repeat red; unfold RelationPairs.RelCompFun in *; simpl in *. 
-  destruct Heqst as [HeqR HeqW]; rewrite Heqr, Heqr1, Heqd; split.
-  - now intro y; rewrite HeqR.
-  - now rewrite HeqW.
-Qed. 
-
-#[export] Instance stock_new_key_eq : Proper (eq ==> Logic.eq) new_key.
-Proof.
-  intros [rt1 wt1] [rt2 wt2] Heq.
-  repeat red in Heq; unfold RelationPairs.RelCompFun in Heq; simpl in *.
-  destruct Heq as [Heqr Heqw].
-  unfold new_key; simpl.
-  now rewrite Heqr, Heqw.
-Qed.
-
-#[export] Instance stock_Empty_iff : Proper (eq ==> iff) Empty.
-Proof.
-  intros [rx wx] [ry wy] [Hreq Hweq].
-  unfold RelationPairs.RelCompFun,Empty in *; simpl in *.
-  rewrite Hreq, Hweq; split; auto.
-Qed.
-
-(** **** [eqDom] properties *)
-
-#[export] Instance eqDom_iff : Proper (RC.eq ==> eq ==> iff) eqDom.
-Proof.
-  intros Rc Rc1 HeqRc W W1 HeqW; unfold eqDom; split; intros.
-  - rewrite <- HeqRc; rewrite <- HeqW; auto.
-  - rewrite HeqRc; rewrite HeqW; auto.
-Qed.
-
-Lemma eqDom_In (r: resource) (Rc: ℜ) (W: t) :
-  eqDom Rc W -> (r ∈ Rc)%rc <-> In r W.
-Proof. unfold eqDom; intro HeqDom; auto. Qed.
-
-Lemma eqDom_Empty (Rc : ℜ) (W: t):
- eqDom Rc W -> (isEmpty(Rc))%rc <-> Empty W.
-Proof.
-  intro HeqDom; split; intro HEmp.
-  - apply Empty_notin; intros r HIn.
-    rewrite <- (eqDom_In r Rc) in HIn; auto.
-    destruct HIn as [v HM].
-    now apply (HEmp r v).
-  - apply Empty_unfold in HEmp.
-    intros x v HM. 
-    apply HEmp.
-    exists x.
-    rewrite <- (eqDom_In x Rc); auto.
-    now exists v.
-Qed.
-
-Lemma eqDom_is_empty (Rc : ℜ) (W: t):
-  eqDom Rc W -> RC.Raw.is_empty Rc = is_empty W.
-Proof.
-  intro HeqDom.
-  destruct (RC.Raw.is_empty Rc) eqn:HisEmp;
-  destruct (is_empty W) eqn:HisEmp'; auto; exfalso.
-  - apply RC.is_empty_2 in HisEmp.
-    rewrite (eqDom_Empty _ W) in HisEmp; auto.
-    now apply not_Empty_is_empty in HisEmp'.
-  - apply Empty_is_empty in HisEmp'.
-    rewrite <- eqDom_Empty in HisEmp'; eauto.
-    apply RC.is_empty_1 in HisEmp'.
-    rewrite HisEmp in *. inversion HisEmp'.
-Qed.
-
-Lemma eqDom_new_key (Rc : ℜ) (W: t):
-  eqDom Rc W -> Rc⁺%rc = new_key W.
-Proof.
-  revert W; induction Rc using RC.map_induction; intros W HeqDom.
-  - rewrite RC.Ext.new_key_Empty; auto.
-    rewrite (eqDom_Empty Rc W HeqDom) in H.
-    rewrite new_key_Empty; auto.
-  - unfold RC.Add in H0; rewrite H0 in *; clear H0.
-    rewrite RC.Ext.new_key_add_max.
-
-    destruct W as [rW wW]; unfold eqDom,In, new_key in *.
-    simpl in HeqDom.
-    simpl (readers (rW, wW)⁺)%sr.
-    simpl (writers (rW, wW)⁺)%rm.
-
-    assert (HIn: (x ∈ ⌈ x ⤆ e ⌉ Rc1)%rc).
-    { rewrite RC.add_in_iff; auto. }
-
-    apply HeqDom in HIn as HIn'.
-    destruct HIn' as [[v HM] | [v' HM']].
-    -- apply SRE.find_1 in HM.
-       apply SRE.add_id in HM; rewrite <- HM; clear HM.
-       rewrite <- SRE.add_remove_1.
-       rewrite SRE.Ext.new_key_add_max.
-
-       destruct (RM.In_dec wW x) as [[v' HM'] | HnInw].
-       + apply RM.find_1 in HM'.
-         apply RM.add_id in HM'; rewrite <- HM'; clear HM'.
-         rewrite <- RM.add_remove_1.
-         rewrite RM.Ext.new_key_add_max.
-         rewrite (IHRc1 (SRE.Raw.remove x rW, RM.Raw.remove x wW)).
-         ++ simpl (readers (SRE.Raw.remove x rW, RM.Raw.remove x wW)).
-            simpl (writers (SRE.Raw.remove x rW, RM.Raw.remove x wW)).
-            lia.
-         ++ intro r; split; simpl.
-            * intro HInRc1.
-              destruct (Resource.eq_dec r x); subst; try contradiction.
-              rewrite SRE.remove_in_iff.
-              rewrite RM.remove_in_iff.
-              rewrite <- RC.add_neq_in_iff in HInRc1; eauto.
-              apply HeqDom in HInRc1 as [|]; auto.
-            * rewrite SRE.remove_in_iff.
-              rewrite RM.remove_in_iff.
-              intros [[Hneq HInr] | [HInw Hneq]].
-              ** rewrite <- RC.add_neq_in_iff; eauto.
-                 rewrite HeqDom; auto.
-              ** rewrite <- RC.add_neq_in_iff; eauto.
-                 rewrite HeqDom; auto.
-       + rewrite (IHRc1 (SRE.Raw.remove x rW, wW)).
-         ++ simpl (readers (SRE.Raw.remove x rW, wW)).
-            simpl (writers (SRE.Raw.remove x rW, wW)).
-            lia.
-         ++ intro r; split; simpl.
-            * intro HInRc1.
-              destruct (Resource.eq_dec r x); subst; try contradiction.
-              rewrite SRE.remove_in_iff.
-              rewrite <- RC.add_neq_in_iff in HInRc1; eauto.
-              apply HeqDom in HInRc1 as [|]; auto.
-            * rewrite SRE.remove_in_iff.
-              intros [[Hneq HInr] | HInw].
-              ** rewrite <- RC.add_neq_in_iff; eauto.
-                 rewrite HeqDom; auto.
-              ** destruct (Resource.eq_dec r x); subst; try contradiction.
-                 rewrite <- RC.add_neq_in_iff; eauto.
-                 rewrite HeqDom; auto.
-    -- apply RM.find_1 in HM'.
-       apply RM.add_id in HM'; rewrite <- HM'; clear HM'.
-       rewrite <- RM.add_remove_1.
-       rewrite RM.Ext.new_key_add_max.
-
-       destruct (SRE.In_dec rW x) as [HInr | HnInr].
-
-       + destruct HInr as [v HM].
-         apply SRE.find_1 in HM.
-         apply SRE.add_id in HM; rewrite <- HM; clear HM.
-         rewrite <- SRE.add_remove_1.
-         rewrite SRE.Ext.new_key_add_max.
-         rewrite (IHRc1 (SRE.Raw.remove x rW, RM.Raw.remove x wW)).
-         ++ simpl (readers (SRE.Raw.remove x rW, RM.Raw.remove x wW)).
-            simpl (writers (SRE.Raw.remove x rW, RM.Raw.remove x wW)).
-            lia.
-         ++ intro r; split; simpl.
-            * intro HInRc1.
-              destruct (Resource.eq_dec r x); subst; try contradiction.
-              rewrite SRE.remove_in_iff.
-              rewrite RM.remove_in_iff.
-              rewrite <- RC.add_neq_in_iff in HInRc1; eauto.
-              apply HeqDom in HInRc1 as [|]; auto.
-            * rewrite SRE.remove_in_iff.
-              rewrite RM.remove_in_iff.
-              intros [[Hneq HInr] | [HInw Hneq]].
-              ** rewrite <- RC.add_neq_in_iff; eauto.
-                 rewrite HeqDom; auto.
-              ** rewrite <- RC.add_neq_in_iff; eauto.
-                 rewrite HeqDom; auto.
-       + rewrite (IHRc1 (rW, RM.Raw.remove x wW)).
-         ++ simpl (readers (rW, RM.Raw.remove x wW)).
-            simpl (writers (rW, RM.Raw.remove x wW)).
-            lia.
-         ++ intro r; split; simpl.
-            * intro HInRc1.
-              destruct (Resource.eq_dec r x); subst; try contradiction.
-              rewrite RM.remove_in_iff.
-              rewrite <- RC.add_neq_in_iff in HInRc1; eauto.
-              apply HeqDom in HInRc1 as [|]; auto.
-            * rewrite RM.remove_in_iff.
-              intros [HInr | [Hneq HInw]].
-              ** destruct (Resource.eq_dec r x); subst; try contradiction.
-                 rewrite <- RC.add_neq_in_iff; eauto.
-                 rewrite HeqDom; auto.
-              ** rewrite <- RC.add_neq_in_iff; eauto.
-                 rewrite HeqDom; auto.
+  induction W; intros HltV HltW.
+  - now simpl.
+  - destruct a as [[rg rs] v].
+    inversion HltW; subst. 
+    simpl in *.
+    destruct (V⌊rs⌋)%re eqn:Hfi.
+    -- destruct r.
+       + constructor; auto.
+         apply IHW; auto.
+       + constructor.
+         ++ apply HltV in Hfi.
+            now simpl in *.
+         ++ apply IHW; auto.
+    -- constructor; auto.
+       apply IHW; auto.
 Qed.
 
 
 (** **** [eqDom] properties *)
+Definition eqDom' (V : 𝐕) (W: t) := forall (r : resource), (r ∈ V)%re <-> In r (keys W).
 
-#[export] Instance eqDom'_iff : Proper (RE.eq ==> eq ==> iff) eqDom'.
+#[export] Instance eqDom'_iff : Proper (REnvironment.eq ==> eq ==> iff) eqDom'.
 Proof.
   intros V V1 HeqV W W1 HeqW; unfold eqDom'; split; intros.
   - rewrite <- HeqV; rewrite <- HeqW; auto.
@@ -1116,207 +382,152 @@ Proof.
 Qed.
 
 Lemma eqDom'_In (r: resource) (V: 𝐕) (W: t) :
-  eqDom' V W -> (r ∈ V)%re <-> In r W.
+  eqDom' V W -> (r ∈ V)%re <-> In r (keys W).
 Proof. unfold eqDom'; intro HeqDom'; auto. Qed.
 
 Lemma eqDom'_Empty (V: 𝐕) (W: t):
- eqDom' V W -> (isEmpty(V))%re <-> Empty W.
+ eqDom' V W -> (isEmpty(V))%re <-> W = [].
 Proof.
   intro HeqDom'; split; intro HEmp.
-  - apply Empty_notin; intros r HIn.
-    rewrite <- (eqDom'_In r V) in HIn; auto.
-    destruct HIn as [v HM].
-    now apply (HEmp r v).
-  - apply Empty_unfold in HEmp.
-    intros x v HM. 
-    apply HEmp.
-    exists x.
-    rewrite <- (eqDom'_In x V); auto.
-    now exists v.
-Qed.
-
-Lemma eqDom'_is_empty (V: 𝐕) (W: t):
-  eqDom' V W -> RE.Raw.is_empty V = is_empty W.
-Proof.
-  intro HeqDom'.
-  destruct (RE.Raw.is_empty V) eqn:HisEmp;
-  destruct (is_empty W) eqn:HisEmp'; auto; exfalso.
-  - apply RE.is_empty_2 in HisEmp.
-    rewrite (eqDom'_Empty _ W) in HisEmp; auto.
-    now apply not_Empty_is_empty in HisEmp'.
-  - apply Empty_is_empty in HisEmp'.
-    rewrite <- eqDom'_Empty in HisEmp'; eauto.
-    apply RE.is_empty_1 in HisEmp'.
-    rewrite HisEmp in *. inversion HisEmp'.
+  - destruct W; auto.
+    destruct p as [[rg rs] v].
+    assert (rg ∈ V)%re.
+    { apply HeqDom'; simpl; auto. }
+    destruct H as [v' HM].
+    exfalso.
+    now apply (HEmp rg v').
+  - subst.
+    intros x v HM.
+    assert (HIn : (x ∈ V)%re).
+    { now exists v. }
+    rewrite (HeqDom' x) in HIn.
+    simpl in *; auto. 
 Qed.
 
 Lemma eqDom'_new_key (V: 𝐕) (W: t):
+  NoDup (keys W) ->
   eqDom' V W -> V⁺%re = new_key W.
 Proof.
-  revert W; induction V using RE.map_induction; intros W HeqDom'.
-  - rewrite RE.Ext.new_key_Empty; auto.
-    rewrite (eqDom'_Empty V W HeqDom') in H.
-    rewrite new_key_Empty; auto.
-  - unfold RE.Add in H0; rewrite H0 in *; clear H0.
-    rewrite RE.Ext.new_key_add_max.
-
-    destruct W as [rW wW]; unfold eqDom',In, new_key in *.
-    simpl in HeqDom'.
-    simpl (readers (rW, wW)⁺)%sr.
-    simpl (writers (rW, wW)⁺)%rm.
-
-    assert (HIn: (x ∈ ⌈ x ⤆ e ⌉ V1)%re).
-    { rewrite RE.add_in_iff; auto. }
-
-    apply HeqDom' in HIn as HIn'.
-    destruct HIn' as [[v HM] | [v' HM']].
-    -- apply SRE.find_1 in HM.
-       apply SRE.add_id in HM; rewrite <- HM; clear HM.
-       rewrite <- SRE.add_remove_1.
-       rewrite SRE.Ext.new_key_add_max.
-
-       destruct (RM.In_dec wW x) as [[v' HM'] | HnInw].
-       + apply RM.find_1 in HM'.
-         apply RM.add_id in HM'; rewrite <- HM'; clear HM'.
-         rewrite <- RM.add_remove_1.
-         rewrite RM.Ext.new_key_add_max.
-         rewrite (IHV1 (SRE.Raw.remove x rW, RM.Raw.remove x wW)).
-         ++ simpl (readers (SRE.Raw.remove x rW, RM.Raw.remove x wW)).
-            simpl (writers (SRE.Raw.remove x rW, RM.Raw.remove x wW)).
-            lia.
-         ++ intro r; split; simpl.
-            * intro HInRc1.
-              destruct (Resource.eq_dec r x); subst; try contradiction.
-              rewrite SRE.remove_in_iff.
-              rewrite RM.remove_in_iff.
-              rewrite <- RE.add_neq_in_iff in HInRc1; eauto.
-              apply HeqDom' in HInRc1 as [|]; auto.
-            * rewrite SRE.remove_in_iff.
-              rewrite RM.remove_in_iff.
-              intros [[Hneq HInr] | [HInw Hneq]].
-              ** rewrite <- RE.add_neq_in_iff; eauto.
-                 rewrite HeqDom'; auto.
-              ** rewrite <- RE.add_neq_in_iff; eauto.
-                 rewrite HeqDom'; auto.
-       + rewrite (IHV1 (SRE.Raw.remove x rW, wW)).
-         ++ simpl (readers (SRE.Raw.remove x rW, wW)).
-            simpl (writers (SRE.Raw.remove x rW, wW)).
-            lia.
-         ++ intro r; split; simpl.
-            * intro HInRc1.
-              destruct (Resource.eq_dec r x); subst; try contradiction.
-              rewrite SRE.remove_in_iff.
-              rewrite <- RE.add_neq_in_iff in HInRc1; eauto.
-              apply HeqDom' in HInRc1 as [|]; auto.
-            * rewrite SRE.remove_in_iff.
-              intros [[Hneq HInr] | HInw].
-              ** rewrite <- RE.add_neq_in_iff; eauto.
-                 rewrite HeqDom'; auto.
-              ** destruct (Resource.eq_dec r x); subst; try contradiction.
-                 rewrite <- RE.add_neq_in_iff; eauto.
-                 rewrite HeqDom'; auto.
-    -- apply RM.find_1 in HM'.
-       apply RM.add_id in HM'; rewrite <- HM'; clear HM'.
-       rewrite <- RM.add_remove_1.
-       rewrite RM.Ext.new_key_add_max.
-
-       destruct (SRE.In_dec rW x) as [HInr | HnInr].
-
-       + destruct HInr as [v HM].
-         apply SRE.find_1 in HM.
-         apply SRE.add_id in HM; rewrite <- HM; clear HM.
-         rewrite <- SRE.add_remove_1.
-         rewrite SRE.Ext.new_key_add_max.
-         rewrite (IHV1 (SRE.Raw.remove x rW, RM.Raw.remove x wW)).
-         ++ simpl (readers (SRE.Raw.remove x rW, RM.Raw.remove x wW)).
-            simpl (writers (SRE.Raw.remove x rW, RM.Raw.remove x wW)).
-            lia.
-         ++ intro r; split; simpl.
-            * intro HInRc1.
-              destruct (Resource.eq_dec r x); subst; try contradiction.
-              rewrite SRE.remove_in_iff.
-              rewrite RM.remove_in_iff.
-              rewrite <- RE.add_neq_in_iff in HInRc1; eauto.
-              apply HeqDom' in HInRc1 as [|]; auto.
-            * rewrite SRE.remove_in_iff.
-              rewrite RM.remove_in_iff.
-              intros [[Hneq HInr] | [HInw Hneq]].
-              ** rewrite <- RE.add_neq_in_iff; eauto.
-                 rewrite HeqDom'; auto.
-              ** rewrite <- RE.add_neq_in_iff; eauto.
-                 rewrite HeqDom'; auto.
-       + rewrite (IHV1 (rW, RM.Raw.remove x wW)).
-         ++ simpl (readers (rW, RM.Raw.remove x wW)).
-            simpl (writers (rW, RM.Raw.remove x wW)).
-            lia.
-         ++ intro r; split; simpl.
-            * intro HInRc1.
-              destruct (Resource.eq_dec r x); subst; try contradiction.
-              rewrite RM.remove_in_iff.
-              rewrite <- RE.add_neq_in_iff in HInRc1; eauto.
-              apply HeqDom' in HInRc1 as [|]; auto.
-            * rewrite RM.remove_in_iff.
-              intros [HInr | [Hneq HInw]].
-              ** destruct (Resource.eq_dec r x); subst; try contradiction.
-                 rewrite <- RE.add_neq_in_iff; eauto.
-                 rewrite HeqDom'; auto.
-              ** rewrite <- RE.add_neq_in_iff; eauto.
-                 rewrite HeqDom'; auto.
+  revert V; induction W; intros V HNoD HeqDom'.
+  - simpl.
+    rewrite REnvironment.Ext.new_key_Empty; auto.
+    rewrite eqDom'_Empty; auto.
+  - destruct a as [[rg rs] v].
+    rewrite new_key_cons.
+    assert (HIn: (rg ∈ V)%re).
+    { rewrite (HeqDom' rg); simpl; auto. }
+    destruct HIn as [v' HM].
+    apply REnvironment.find_1 in HM.
+    apply REnvironment.add_id in HM.
+    rewrite <- HM in *; clear HM.
+    rewrite <- REnvironment.add_remove_1 in *.
+    assert (HIn: (rs ∈ (⌈ rg ⤆ v' ⌉ REnvironment.Raw.remove rg V))%re).
+    { rewrite (HeqDom' rs); simpl; auto. }
+    destruct HIn as [v'' HM].
+    apply REnvironment.find_1 in HM.
+    apply REnvironment.add_id in HM.
+    rewrite <- HM in *; clear HM.
+    rewrite <- REnvironment.add_remove_1 in *.
+    inversion HNoD; subst; simpl in *.
+    inversion H2; subst; simpl in *.
+    clear H2 HNoD; simpl in *.
+    apply Classical_Prop.not_or_and in H1 as [Hneq HnIn].
+    rewrite REnvironment.remove_add_2 in * by lia.
+    do 2 rewrite REnvironment.Ext.new_key_add_max.
+    rewrite IHW; try lia; auto.
+    intros r; split; intro HIn.
+    + assert (HIn': (r ∈ (⌈ rs ⤆ v'' ⌉ (⌈ rg ⤆ v' ⌉ REnvironment.Raw.remove rs (REnvironment.Raw.remove rg V))))%re).
+      { do 2 rewrite REnvironment.add_in_iff; auto. }
+      apply HeqDom' in HIn'.
+      apply REnvironment.remove_in_iff in HIn as [Hneq' HIn].
+      apply REnvironment.remove_in_iff in HIn as [Hneq'' HIn].
+      simpl in HIn'; destruct HIn' as [Hc|[Hc|]]; auto;
+      subst; try contradiction.
+    + assert (In r (keys ((rg,rs,v):: W))).
+      { simpl; auto. }
+      apply HeqDom' in H.
+      do 2 rewrite REnvironment.add_in_iff in H.
+      destruct H as [Hc|[Hc|HIn']]; subst; try contradiction; auto.
 Qed.
 
 
+Lemma init_locals_in_iff (r : resource) (W : t) (V : 𝐕) :
+  (r ∈ (init_locals W V))%re <-> In r (keys W) \/ (r ∈ V)%re.
+Proof.
+  revert r; induction W; simpl; intros r.
+  - split; intros; auto.
+    destruct H; auto.
+    contradiction.
+  - destruct a as [[rg rs] v]; split; intro HIn.
+    -- do 2 rewrite REnvironment.add_in_iff in HIn.
+       simpl.
+       destruct HIn as [|[| HIn]]; subst; auto.
+       apply IHW in HIn as [|]; auto.
+    -- simpl in *.
+       do 2 rewrite REnvironment.add_in_iff.
+       rewrite IHW.
+       destruct HIn as [[|[|]]|]; auto; subst.
+Qed.
+
+Lemma init_locals_new_key (V : 𝐕) (t : t) : ((init_locals t V)⁺)%re = max (new_key t) (V⁺)%re.
+Proof.
+  induction t; auto.
+  destruct a as [[rg rs] v].
+  rewrite new_key_cons.
+  simpl.
+  do 2 rewrite REnvironment.Ext.new_key_add_max.
+  rewrite IHt; lia.
+Qed.
+
+Lemma init_locals_Wf (k : lvl) (V : 𝐕) (t : t) :
+  Wf k t /\ (k ⊩ V)%re -> (k ⊩ init_locals t V)%re.
+Proof.
+  induction t; simpl; intros [Hwf Hwf']; auto.
+  destruct a as [[rg rs] v].
+  apply Wf_cons in Hwf as [Hwf Hwf''].
+  destruct Hwf as [Hwfrg [Hwfrs Hwfv]].
+  apply REnvironment.Wf_add; split; auto.
+  split.
+  - now unfold Cell.Wf; simpl.
+  - apply REnvironment.Wf_add; repeat split; auto.
+    constructor.
+Qed.
+
+Lemma init_locals_find_e r c  (V : 𝐕) (W : t) :
+  (V⌊r⌋%re = Some c -> exists v, Logic.eq c (Cell.inp v)) ->
+  (init_locals W V)⌊r⌋%re = Some c -> exists v, Logic.eq c (Cell.inp v).
+Proof.
+  revert r c; induction W; intros r c Hfi.
+  - simpl; auto.
+  - destruct a as [[rg rs] v].
+    simpl.
+    intro Hfi'.
+    rewrite REnvironment.add_o in Hfi'.
+    destruct (Resource.eq_dec rg r); subst.
+    -- now inversion Hfi'; exists v.
+    -- rewrite REnvironment.add_o in Hfi'.
+       destruct (Resource.eq_dec rs r); subst.
+       + inversion Hfi'; subst.
+         now exists <[unit]>.
+       + eapply IHW; eauto.
+Qed.
+
 End Stock.
 
-(** ---- *)
-
-(** ** Notation - Virtual Resource Environment *)
-
 Module StockNotations.
-
-(** *** Scope *)
+  (** *** Scope *)
 Declare Scope stock_scope.
 Delimit Scope stock_scope with sk.
 
 (** *** Notations *)
 Definition 𝐖 := Stock.t.
 
-Infix "∈" := Stock.In (at level 60, no associativity) : stock_scope. 
-Notation "r '∉' t" := (~ (Stock.In r t)) (at level 75, no associativity) : stock_scope. 
+Infix "∈" := List.In (at level 60, no associativity) : stock_scope. 
+Notation "r '∉' t" := (~ (List.In r t)) (at level 75, no associativity) : stock_scope. 
 Notation "t '⁺'" := (Stock.new_key t) (at level 16) : stock_scope.
-Notation "∅" := Stock.empty (at level 0, no associativity) : stock_scope. 
-Notation "t '⌊' x '⌋'"  := (Stock.find x t) (at level 15, x constr) : stock_scope.
-Notation "⌈ x '~' x1 ⤆ v '⌉' t"  := (Stock.add x x1 v t) 
-                                     (at level 15, x constr, v constr) : stock_scope.
 Notation "'[⧐' lb '–' k ']' t" := (Stock.shift lb k t) 
                                    (at level 65, right associativity) : stock_scope.
 
 Infix "=" := Stock.eq : stock_scope.
-Infix "∪" := Stock.union : stock_scope.
 Infix "⊩" := Stock.Wf (at level 20, no associativity) : stock_scope.
-
-(** *** Morphisms *)
-
-Import Stock.
-
-#[export] Instance stock_shift_eq : Proper (Resource.eq ==> Resource.eq ==> eq ==> eq) shift := _.
-
-#[export] Instance stock_Wf_iff : Proper (Resource.eq ==> eq ==> iff) Wf := _.
-
-#[export] Instance stock_halts_iff: Proper (Logic.eq ==> eq ==> iff) halts := _.
-
-#[export] Instance stock_in_iff : Proper (Logic.eq ==> eq ==> iff) In := _.
-
-#[export] Instance stock_find_eq : Proper (Logic.eq ==> eq ==> Logic.eq) find := _.
-
-#[export] Instance stock_add_eq : 
-  Proper (Resource.eq ==> Resource.eq ==> Term.eq ==> eq ==> eq) add := _.
-
-#[export] Instance stock_new_key_eq : Proper (eq ==> Logic.eq) new_key := _.
-
-#[export] Instance stock_Empty_iff : Proper (eq ==> iff) Empty := _.
-
-#[export] Instance stock_eqDom_iff : Proper (RC.eq ==> eq ==> iff) eqDom := _.
-
-#[export] Instance stock_eqDom'_iff : Proper (RE.eq ==> eq ==> iff) eqDom' := _.
-
 End StockNotations.
